@prefix rdfs: <http://www.w3.org/2000/01/rdf-schema#>.
@prefix rdf: <http://www.w3.org/1999/02/22-rdf-syntax-ns#>.
@prefix xsd: <http://www.w3.org/2001/XMLSchema#>.
@prefix qprob: <http://purl.org/eis/vocab/qprob#>.
@prefix owl: <http://www.w3.org/2002/07/owl#>.
@prefix daq: <http://purl.org/eis/vocab/daq#>.
@prefix qr: <http://purl.org/eis/vocab/qr#>.
@prefix dqm: <http://purl.org/eis/vocab/dqm#>.

	
qprob:CleaningRecommendation a rdfs:Class ;
	rdfs:comment "Represents recommendation for how to solve the corresponding quality problem." ;
	rdfs:label "Cleaning Suggestion" .
	
	
qprob:MalformedDatatypeLiteralsProblem a rdfs:Class ;
	rdfs:subClassOf qr:QualityProblem ;
	rdfs:comment "Represents a kind of quality problems in which literal value is not consistent with defined data type" ;
	qprob:problemDescription "Literal value is not consistent with the defined data type.";
	qprob:cleaningSuggestion "Parse or convert literal into the value space of the data type." ;
	qr:identifiedBy dqm:MalformedDatatypeLiteralsMetric;
	rdfs:label "Malformed Datatype literals Problem" . 
	
qprob:IncompatibleDatatypeRangeProblem a rdfs:Class ;
	rdfs:subClassOf qr:QualityProblem ;
	rdfs:comment "Represents a kind of quality problems in which literal value is not consistent with data type defined by property range" ; 
	qprob:problemDescription "Literal value is not consistent with data type defined by property range" ;
	qprob:cleaningSuggestion "Parse or convert the literal value into the value space of the range datatype" ;
	qr:identifiedBy dqm:IncompatibleDatatypeRangeMetric;
	rdfs:label "Incompatible Datatype Range Problem " . 
	

qprob:HomogeneousDatatypesProblem a rdfs:Class ;
	rdfs:subClassOf qr:QualityProblem ;
	qprob:problemDescription "Data type of literals corresponding to the same property is not homogeneous" ;
	qprob:cleaningSuggestion "Parse or convert literal values to unique data type" ;
	rdfs:comment "Represents a kind of quality problems in which data type are not homogeneous" ;
	qr:identifiedBy dqm:HomogeneousDatatypesMetric;
	rdfs:label "Homogeneous Datatype Problem " . 
	

qprob:MisplacedClassesOrPropertiesProblem a rdfs:Class ;
	rdfs:subClassOf qr:QualityProblem ;
	rdfs:comment "Represents a kind of quality problems in which classes or properties is not places properly." ;
	qr:identifiedBy dqm:MisplacedClassesOrPropertiesMetric;
	rdfs:label "Misplaced classes or properties Problem " . 
	
qprob:MisplacedClassProblem a rdfs:Class ;
	rdfs:subClassOf qprob:MisplacedClassesOrPropertiesProblem ;
	rdfs:comment "Represents a kind of quality problems in which classes is not places properly." ;
	qprob:problemDescription "Class is used in the property position" ;
	qprob:cleaningSuggestion "Define an appropriate property" ;
	rdfs:label "Misplaced classes Problem " . 
	
qprob:MisplacedPropertyProblem a rdfs:Class ;
	rdfs:subClassOf qprob:MisplacedClassesOrPropertiesProblem ;
	rdfs:comment "Represents a kind of quality problems in which property is not places properly." ;
	qprob:problemDescription "Property is used in a class position" ;
	qprob:cleaningSuggestion "Define an appropriate class" ;
	rdfs:label "Misplaced Property Problem " . 
	

qprob:MisuseOwlDatatypeOrObjectPropertiesProblem a rdfs:Class ;
	rdfs:subClassOf qr:QualityProblem ;
	rdfs:comment "Represents a kind of quality problems in which properties are not used properly." ;
	qr:identifiedBy dqm:MisusedOwlDatatypeOrObjectPropertiesMetric;
	rdfs:label "Misuse Owl Datatype Or Object Properties Problem" .
	
	
qprob:MisuseOwlDatatypePropertyProblem a rdfs:Class ;
	rdfs:subClassOf qprob:MisuseOwlDatatypeOrObjectPropertiesProblem ;
	rdfs:comment "Represents a kind of quality problems in which the property of the class  owl:DatatypeProperty is used as owl:ObjectProperty." ;
	qprob:problemDescription "The property of the class owl:ObjectProperty points to a literal" ;
	qprob:cleaningSuggestion "Use class of owl:DatatypeProperty or change object to rdfs:Resource" ;
	rdfs:label "Misuse Owl Datatype Property Problem" .
	
qprob:MisuseOwlDatatypePropertyProblem a rdfs:Class ;
	rdfs:subClassOf qprob:MisuseOwlDatatypeOrObjectPropertiesProblem ;
	rdfs:comment "Represents a kind of quality problems in which the property of the class owl:ObjectProperty is used as owl:DatatypeProperty." ;
	qprob:problemDescription "The property of the class owl:DatatypeProperty points to a ressource" ;
	qprob:cleaningSuggestion "Use class of owl:ObjectProperty or change object to rdfs:Literal" ;
	rdfs:label "Misuse Owl ObjectProperty Problem" .
	

qprob:UndefinedClassesProblem a rdfs:Class ;
	rdfs:subClassOf qr:QualityProblem ;
	qprob:problemDescription "Class is not defined." ;
	rdfs:comment "Represents a kind of quality problems in which classes are not defined" ;
	qprob:cleaningSuggestion "Use a defined class. " ;
	qr:identifiedBy dqm:UndefinedClassesMetric;
	rdfs:label "Undefined Classes Problem" .
	
qprob:UndefinedPropertiesProblem a rdfs:Class ;
	rdfs:subClassOf qr:QualityProblem ;
	qprob:problemDescription "Property is not defined." ;
	qprob:cleaningSuggestion "Use a defined property." ;
	rdfs:comment "Represents a kind of quality problems in which classes or properties are not defined" ;
	qr:identifiedBy dqm:UndefinedPropertiesMetric;
	rdfs:label "Undefined Properties Problem".
	
	
qprob:WhitespaceInAnnotationProblem a rdfs:Class ;
	rdfs:subClassOf qr:QualityProblem ;
	qprob:problemDescription "Literal value contains white spaces";
	qprob:cleaningSuggestion "Trim leading and trailing whitespace" ;
	rdfs:comment "Represents a kind of quality problems in which object in annotation property contains white spaces." ;
	qprob:qrefineRule "";
	qr:identifiedBy dqm:WhitespaceInAnnotationMetric;
	rdfs:label "Whitespace in Annotation Problem".
	
	
qprob:OntologyHijackingProblem a rdfs:Class ;
	rdfs:subClassOf qr:QualityProblem ;
	qprob:problemDescription "The triple hijackes an existing ontology";
	qprob:cleaningSuggestion " " ;
	rdfs:comment "Represents a kind of quality problems in the a statement hijackes an existing ontology." ;
	qprob:qrefineRule "";
	qr:identifiedBy dqm:OntologyHijackingMetric;
	rdfs:label "Ontology Hijacking Problem".
	

qprob:EmptyAnnotationValueProblem a rdfs:Class ;
	rdfs:subClassOf qr:QualityProblem ;
	rdfs:comment "Represents a kind of quality problems in which literal value in annotation property is empty." ;
	qprob:problemDescription "Literal value is empty";
	qprob:cleaningSuggestion "Remove the triple or add literal value" ;
	qr:identifiedBy dqm:EmptyAnnotationValueMetric;
	rdfs:label "Empty Annotation Value Problem".
	
	
qprob:LabelsUsingCapitalsProblem a rdfs:Class ;
	rdfs:subClassOf qr:QualityProblem ;
	rdfs:comment "Represents a kind of quality problems in which object value in label property uses a bad style of capitalization." ;
	qprob:problemDescription "Literal uses a bad style of capitalization";
	qprob:cleaningSuggestion "Change the capitalization of the literal";
	qprob:qrefineRule "";
	qr:identifiedBy dqm:LabelsUsingCapitalsMetric;
	rdfs:label "Labels Using Capitals Problem".
	
	
qprob:BlankNodeUsageProblem a rdfs:Class ;
	rdfs:subClassOf qr:QualityProblem ;	
	rdfs:comment "Represents a kind of quality problems in which blank nodes are used in subject or object position." ;	
	qr:identifiedBy dqm:LowBlankNodesUsageMetric;
	rdfs:label "Blank Node Usage Problem".
	
qprob:BlankNodeObjectProblem a rdfs:Class ;
	rdfs:subClassOf qr:QualityProblem ;
	qprob:problemDescription "The triple contains a blank node";
	rdfs:comment "Represents a kind of quality problems in which blank nodes are used in subject or object position." ;
	qprob:cleaningSuggestion "Assign an URI to the node";
	rdfs:label "Blank Node Usage Problem".
	

qprob:RDFAccessibilityProblem a rdfs:Class ;
	rdfs:subClassOf qr:QualityProblem ;
	qprob:problemDescription "RDF dump is not available";
	rdfs:comment "Represents a kind of quality problems when RDF can not be accessed." ;
	qprob:cleaningSuggestion "Check the path to RDF dump or remove the triple";
	rdfs:label "RDF Accessibility Problem".
	
	
qprob:SPARQLAccessibilityProblem a rdfs:Class ;
	rdfs:subClassOf qr:QualityProblem ;
	qprob:problemDescription "SPARQL Endpoint is not accessible";
	rdfs:comment "Represents a kind of quality problems when SPARQL Endpoint can not be accessed." ;
	qprob:cleaningSuggestion "Check the SPARQL Endpoint  URI or remove the triple";
	rdfs:label "SPARQL Accessibility Problem".
	
		

	
	
# Properties


	
	
qr:problemDescription
		a	rdf:Property, owl:DatatypeProperty ;
		rdfs:label	"problemDescription" ;
		rdfs:comment	"Contains brief summary of the quality problem that is presented to the user." ;
		rdfs:domain	qr:QualityProblem;
		rdfs:range	 xsd:string.
		
qr:cleaningSuggestion
		a	rdf:Property, owl:DatatypeProperty ;
		rdfs:label	"recommendation" ;
		rdfs:comment	"Contains recommendation of how to solve the corresponding quality problem." ;
		rdfs:domain	qr:QualityProblem;
		rdfs:range	 xsd:string.

		
qr:qrefineRule
		a	rdf:Property, owl:DatatypeProperty ;
		rdfs:label	"recommendation" ;
		rdfs:comment	"Contains cleaning rule for the corresponding quality problem in OpenRefine language." ;
		rdfs:domain	qr:QualityProblem;
		rdfs:range	 xsd:string.

		