<?xml version="1.0" encoding="UTF-8"?>
<rdf:RDF
   xmlns:qprob="http://purl.org/eis/vocab/qprob#"
   xmlns:qr="http://purl.org/eis/vocab/qr#"
   xmlns:rdf="http://www.w3.org/1999/02/22-rdf-syntax-ns#"
   xmlns:rdfs="http://www.w3.org/2000/01/rdf-schema#"
>
  <rdf:Description rdf:about="http://purl.org/eis/vocab/qprob#LabelsUsingCapitalsProblem">
    <rdf:type rdf:resource="http://www.w3.org/2000/01/rdf-schema#Class"/>
    <rdfs:subClassOf rdf:resource="http://purl.org/eis/vocab/qr#QualityProblem"/>
    <rdfs:comment>Represents a kind of quality problems in which object value in label property uses a bad style of capitalization.</rdfs:comment>
    <qprob:qrefineRule></qprob:qrefineRule>
    <rdfs:label>Labels Using Capitals Problem</rdfs:label>
    <qr:identifiedBy rdf:resource="http://purl.org/eis/vocab/dqm#LabelsUsingCapitalsMetric"/>
    <qprob:cleaningSuggestion>Change the capitalization of the literal</qprob:cleaningSuggestion>
    <qprob:problemDescription>Literal uses a bad style of capitalization</qprob:problemDescription>
  </rdf:Description>
  <rdf:Description rdf:about="http://purl.org/eis/vocab/qprob#HomogeneousDatatypesProblem">
    <qr:identifiedBy rdf:resource="http://purl.org/eis/vocab/dqm#HomogeneousDatatypesMetric"/>
    <qprob:cleaningSuggestion>Parse or convert literal values to unique data type</qprob:cleaningSuggestion>
    <qprob:problemDescription>Data type of literals corresponding to the same property is not homogeneous</qprob:problemDescription>
    <rdfs:label>Homogeneous Datatype Problem </rdfs:label>
    <rdfs:comment>Represents a kind of quality problems in which data type are not homogeneous</rdfs:comment>
    <rdfs:subClassOf rdf:resource="http://purl.org/eis/vocab/qr#QualityProblem"/>
    <rdf:type rdf:resource="http://www.w3.org/2000/01/rdf-schema#Class"/>
  </rdf:Description>
  <rdf:Description rdf:about="http://purl.org/eis/vocab/qprob#EmptyAnnotationValueProblem">
    <rdfs:subClassOf rdf:resource="http://purl.org/eis/vocab/qr#QualityProblem"/>
    <qprob:cleaningSuggestion>Remove the triple or add literal value</qprob:cleaningSuggestion>
    <qr:identifiedBy rdf:resource="http://purl.org/eis/vocab/dqm#EmptyAnnotationValueMetric"/>
    <rdfs:label>Empty Annotation Value Problem</rdfs:label>
    <rdf:type rdf:resource="http://www.w3.org/2000/01/rdf-schema#Class"/>
    <rdfs:comment>Represents a kind of quality problems in which literal value in annotation property is empty.</rdfs:comment>
    <qprob:problemDescription>Literal value is empty</qprob:problemDescription>
  </rdf:Description>
  <rdf:Description rdf:about="http://purl.org/eis/vocab/qr#problemDescription">
    <rdfs:domain rdf:resource="http://purl.org/eis/vocab/qr#QualityProblem"/>
    <rdf:type rdf:resource="http://www.w3.org/2002/07/owl#DatatypeProperty"/>
    <rdfs:range rdf:resource="http://www.w3.org/2001/XMLSchema#string"/>
    <rdfs:label>problemDescription</rdfs:label>
    <rdfs:comment>Contains brief summary of the quality problem that is presented to the user.</rdfs:comment>
    <rdf:type rdf:resource="http://www.w3.org/1999/02/22-rdf-syntax-ns#Property"/>
  </rdf:Description>
  <rdf:Description rdf:about="http://purl.org/eis/vocab/qprob#IncompatibleDatatypeRangeProblem">
    <rdfs:comment>Represents a kind of quality problems in which literal value is not consistent with data type defined by property range</rdfs:comment>
    <qprob:cleaningSuggestion>Parse or convert the literal value into the value space of the range datatype</qprob:cleaningSuggestion>
    <rdfs:subClassOf rdf:resource="http://purl.org/eis/vocab/qr#QualityProblem"/>
    <rdf:type rdf:resource="http://www.w3.org/2000/01/rdf-schema#Class"/>
    <rdfs:label>Incompatible Datatype Range Problem </rdfs:label>
    <qr:identifiedBy rdf:resource="http://purl.org/eis/vocab/dqm#IncompatibleDatatypeRangeMetric"/>
    <qprob:problemDescription>Literal value is not consistent with data type defined by property range</qprob:problemDescription>
  </rdf:Description>
  <rdf:Description rdf:about="http://purl.org/eis/vocab/qprob#MisplacedClassesOrPropertiesProblem">
    <rdfs:subClassOf rdf:resource="http://purl.org/eis/vocab/qr#QualityProblem"/>
    <rdfs:comment>Represents a kind of quality problems in which classes or properties is not places properly.</rdfs:comment>
    <rdf:type rdf:resource="http://www.w3.org/2000/01/rdf-schema#Class"/>
    <rdfs:label>Misplaced classes or properties Problem </rdfs:label>
    <qr:identifiedBy rdf:resource="http://purl.org/eis/vocab/dqm#MisplacedClassesOrPropertiesMetric"/>
  </rdf:Description>
  <rdf:Description rdf:about="http://purl.org/eis/vocab/qprob#MisuseOwlDatatypeOrObjectPropertiesProblem">
    <rdf:type rdf:resource="http://www.w3.org/2000/01/rdf-schema#Class"/>
    <rdfs:label>Misuse Owl Datatype Or Object Properties Problem</rdfs:label>
    <rdfs:comment>Represents a kind of quality problems in which properties are not used properly.</rdfs:comment>
    <rdfs:subClassOf rdf:resource="http://purl.org/eis/vocab/qr#QualityProblem"/>
    <qr:identifiedBy rdf:resource="http://purl.org/eis/vocab/dqm#MisusedOwlDatatypeOrObjectPropertiesMetric"/>
  </rdf:Description>
  <rdf:Description rdf:about="http://purl.org/eis/vocab/qprob#MisplacedPropertyProblem">
    <qprob:problemDescription>Property is used in a class position</qprob:problemDescription>
    <rdfs:comment>Represents a kind of quality problems in which property is not places properly.</rdfs:comment>
    <rdfs:label>Misplaced Property Problem </rdfs:label>
    <rdf:type rdf:resource="http://www.w3.org/2000/01/rdf-schema#Class"/>
    <qprob:cleaningSuggestion>Define an appropriate class</qprob:cleaningSuggestion>
    <rdfs:subClassOf rdf:resource="http://purl.org/eis/vocab/qprob#MisplacedClassesOrPropertiesProblem"/>
  </rdf:Description>
  <rdf:Description rdf:about="http://purl.org/eis/vocab/qprob#CleaningRecommendation">
    <rdf:type rdf:resource="http://www.w3.org/2000/01/rdf-schema#Class"/>
    <rdfs:comment>Represents recommendation for how to solve the corresponding quality problem.</rdfs:comment>
    <rdfs:label>Cleaning Suggestion</rdfs:label>
  </rdf:Description>
  <rdf:Description rdf:about="http://purl.org/eis/vocab/qprob#WhitespaceInAnnotationProblem">
    <qr:identifiedBy rdf:resource="http://purl.org/eis/vocab/dqm#WhitespaceInAnnotationMetric"/>
    <rdfs:comment>Represents a kind of quality problems in which object in annotation property contains white spaces.</rdfs:comment>
    <qprob:problemDescription>Literal value contains white spaces</qprob:problemDescription>
    <qprob:qrefineRule></qprob:qrefineRule>
    <rdf:type rdf:resource="http://www.w3.org/2000/01/rdf-schema#Class"/>
    <rdfs:subClassOf rdf:resource="http://purl.org/eis/vocab/qr#QualityProblem"/>
    <rdfs:label>Whitespace in Annotation Problem</rdfs:label>
    <qprob:cleaningSuggestion>Trim leading and trailing whitespace</qprob:cleaningSuggestion>
  </rdf:Description>
  <rdf:Description rdf:about="http://purl.org/eis/vocab/qr#qrefineRule">
    <rdfs:domain rdf:resource="http://purl.org/eis/vocab/qr#QualityProblem"/>
    <rdf:type rdf:resource="http://www.w3.org/2002/07/owl#DatatypeProperty"/>
    <rdfs:comment>Contains cleaning rule for the corresponding quality problem in OpenRefine language.</rdfs:comment>
    <rdfs:label>recommendation</rdfs:label>
    <rdf:type rdf:resource="http://www.w3.org/1999/02/22-rdf-syntax-ns#Property"/>
    <rdfs:range rdf:resource="http://www.w3.org/2001/XMLSchema#string"/>
  </rdf:Description>
  <rdf:Description rdf:about="http://purl.org/eis/vocab/qprob#MalformedDatatypeLiteralsProblem">
    <rdfs:subClassOf rdf:resource="http://purl.org/eis/vocab/qr#QualityProblem"/>
    <qprob:problemDescription>Literal value is not consistent with the defined data type.</qprob:problemDescription>
    <qprob:cleaningSuggestion>Parse or convert literal into the value space of the data type.</qprob:cleaningSuggestion>
    <qr:identifiedBy rdf:resource="http://purl.org/eis/vocab/dqm#MalformedDatatypeLiteralsMetric"/>
    <rdf:type rdf:resource="http://www.w3.org/2000/01/rdf-schema#Class"/>
    <rdfs:label>Malformed Datatype literals Problem</rdfs:label>
    <rdfs:comment>Represents a kind of quality problems in which literal value is not consistent with defined data type</rdfs:comment>
  </rdf:Description>
  <rdf:Description rdf:about="http://purl.org/eis/vocab/qprob#BlankNodeObjectProblem">
    <rdfs:comment>Represents a kind of quality problems in which blank nodes are used in subject or object position.</rdfs:comment>
    <rdfs:label>Blank Node Usage Problem</rdfs:label>
    <qprob:problemDescription>The triple contains a blank node</qprob:problemDescription>
    <qprob:cleaningSuggestion>Assign an URI to the node</qprob:cleaningSuggestion>
    <rdfs:subClassOf rdf:resource="http://purl.org/eis/vocab/qr#QualityProblem"/>
    <rdf:type rdf:resource="http://www.w3.org/2000/01/rdf-schema#Class"/>
  </rdf:Description>
  <rdf:Description rdf:about="http://purl.org/eis/vocab/qprob#BlankNodeUsageProblem">
    <rdfs:comment>Represents a kind of quality problems in which blank nodes are used in subject or object position.</rdfs:comment>
    <qr:identifiedBy rdf:resource="http://purl.org/eis/vocab/dqm#LowBlankNodesUsageMetric"/>
    <rdf:type rdf:resource="http://www.w3.org/2000/01/rdf-schema#Class"/>
    <rdfs:label>Blank Node Usage Problem</rdfs:label>
    <rdfs:subClassOf rdf:resource="http://purl.org/eis/vocab/qr#QualityProblem"/>
  </rdf:Description>
  <rdf:Description rdf:about="http://purl.org/eis/vocab/qprob#RDFAccessibilityProblem">
    <rdf:type rdf:resource="http://www.w3.org/2000/01/rdf-schema#Class"/>
    <rdfs:label>RDF Accessibility Problem</rdfs:label>
    <rdfs:subClassOf rdf:resource="http://purl.org/eis/vocab/qr#QualityProblem"/>
    <qprob:cleaningSuggestion>Check the path to RDF dump or remove the triple</qprob:cleaningSuggestion>
    <rdfs:comment>Represents a kind of quality problems when RDF can not be accessed.</rdfs:comment>
    <qprob:problemDescription>RDF dump is not available</qprob:problemDescription>
  </rdf:Description>
  <rdf:Description rdf:about="http://purl.org/eis/vocab/qr#cleaningSuggestion">
    <rdfs:label>recommendation</rdfs:label>
    <rdfs:comment>Contains recommendation of how to solve the corresponding quality problem.</rdfs:comment>
    <rdf:type rdf:resource="http://www.w3.org/1999/02/22-rdf-syntax-ns#Property"/>
    <rdfs:domain rdf:resource="http://purl.org/eis/vocab/qr#QualityProblem"/>
    <rdfs:range rdf:resource="http://www.w3.org/2001/XMLSchema#string"/>
    <rdf:type rdf:resource="http://www.w3.org/2002/07/owl#DatatypeProperty"/>
  </rdf:Description>
  <rdf:Description rdf:about="http://purl.org/eis/vocab/qprob#MisplacedClassProblem">
    <rdfs:label>Misplaced classes Problem </rdfs:label>
    <qprob:problemDescription>Class is used in the property position</qprob:problemDescription>
    <qprob:cleaningSuggestion>Define an appropriate property</qprob:cleaningSuggestion>
    <rdf:type rdf:resource="http://www.w3.org/2000/01/rdf-schema#Class"/>
    <rdfs:comment>Represents a kind of quality problems in which classes is not places properly.</rdfs:comment>
    <rdfs:subClassOf rdf:resource="http://purl.org/eis/vocab/qprob#MisplacedClassesOrPropertiesProblem"/>
  </rdf:Description>
  <rdf:Description rdf:about="http://purl.org/eis/vocab/qprob#UndefinedClassesProblem">
    <qprob:cleaningSuggestion>Use a defined class. </qprob:cleaningSuggestion>
    <rdfs:subClassOf rdf:resource="http://purl.org/eis/vocab/qr#QualityProblem"/>
    <rdfs:label>Undefined Classes Problem</rdfs:label>
    <qprob:problemDescription>Class is not defined.</qprob:problemDescription>
    <rdf:type rdf:resource="http://www.w3.org/2000/01/rdf-schema#Class"/>
    <qr:identifiedBy rdf:resource="http://purl.org/eis/vocab/dqm#UndefinedClassesMetric"/>
    <rdfs:comment>Represents a kind of quality problems in which classes are not defined</rdfs:comment>
  </rdf:Description>
  <rdf:Description rdf:about="http://purl.org/eis/vocab/qprob#OntologyHijackingProblem">
    <rdfs:label>Ontology Hijacking Problem</rdfs:label>
    <rdf:type rdf:resource="http://www.w3.org/2000/01/rdf-schema#Class"/>
    <qprob:qrefineRule></qprob:qrefineRule>
    <rdfs:comment>Represents a kind of quality problems in the a statement hijackes an existing ontology.</rdfs:comment>
    <rdfs:subClassOf rdf:resource="http://purl.org/eis/vocab/qr#QualityProblem"/>
    <qprob:cleaningSuggestion> </qprob:cleaningSuggestion>
    <qprob:problemDescription>The triple hijackes an existing ontology</qprob:problemDescription>
    <qr:identifiedBy rdf:resource="http://purl.org/eis/vocab/dqm#OntologyHijackingMetric"/>
  </rdf:Description>
  <rdf:Description rdf:about="http://purl.org/eis/vocab/qprob#SPARQLAccessibilityProblem">
    <rdfs:label>SPARQL Accessibility Problem</rdfs:label>
    <rdf:type rdf:resource="http://www.w3.org/2000/01/rdf-schema#Class"/>
    <qprob:problemDescription>SPARQL Endpoint is not accessible</qprob:problemDescription>
    <rdfs:subClassOf rdf:resource="http://purl.org/eis/vocab/qr#QualityProblem"/>
    <rdfs:comment>Represents a kind of quality problems when SPARQL Endpoint can not be accessed.</rdfs:comment>
    <qprob:cleaningSuggestion>Check the SPARQL Endpoint  URI or remove the triple</qprob:cleaningSuggestion>
  </rdf:Description>
  <rdf:Description rdf:about="http://purl.org/eis/vocab/qprob#MisuseOwlDatatypePropertyProblem">
    <rdfs:comment>Represents a kind of quality problems in which the property of the class  owl:DatatypeProperty is used as owl:ObjectProperty.</rdfs:comment>
    <rdfs:label>Misuse Owl ObjectProperty Problem</rdfs:label>
    <rdfs:label>Misuse Owl Datatype Property Problem</rdfs:label>
    <qprob:cleaningSuggestion>Use class of owl:DatatypeProperty or change object to rdfs:Resource</qprob:cleaningSuggestion>
    <rdfs:subClassOf rdf:resource="http://purl.org/eis/vocab/qprob#MisuseOwlDatatypeOrObjectPropertiesProblem"/>
    <rdf:type rdf:resource="http://www.w3.org/2000/01/rdf-schema#Class"/>
    <qprob:cleaningSuggestion>Use class of owl:ObjectProperty or change object to rdfs:Literal</qprob:cleaningSuggestion>
    <qprob:problemDescription>The property of the class owl:DatatypeProperty points to a ressource</qprob:problemDescription>
    <qprob:problemDescription>The property of the class owl:ObjectProperty points to a literal</qprob:problemDescription>
    <rdfs:comment>Represents a kind of quality problems in which the property of the class owl:ObjectProperty is used as owl:DatatypeProperty.</rdfs:comment>
  </rdf:Description>
  <rdf:Description rdf:about="http://purl.org/eis/vocab/qprob#UndefinedPropertiesProblem">
    <rdfs:label>Undefined Properties Problem</rdfs:label>
    <qprob:cleaningSuggestion>Use a defined property.</qprob:cleaningSuggestion>
    <rdfs:subClassOf rdf:resource="http://purl.org/eis/vocab/qr#QualityProblem"/>
    <rdf:type rdf:resource="http://www.w3.org/2000/01/rdf-schema#Class"/>
    <qprob:problemDescription>Property is not defined.</qprob:problemDescription>
    <rdfs:comment>Represents a kind of quality problems in which classes or properties are not defined</rdfs:comment>
    <qr:identifiedBy rdf:resource="http://purl.org/eis/vocab/dqm#UndefinedPropertiesMetric"/>
  </rdf:Description>
</rdf:RDF>